src/Find_proof_2.thy
@@ -11,6 +11,93 @@ declare ts_to_ms_def_2[simp] (* likely a simp *)
 declare dest_fts_focus_def_2[simp] (* surely a simp *)
 declare dest_cnode_t_def_2[simp]
 
+lemma tree_to_leaves_node_eq: "Node(ks,rs) |> tree_to_leaves = rs|>(List.map tree_to_leaves)|>List.concat"
+apply(force intro:FIXME)
+done
+
+
+lemma "lem9"
+apply(simp add: lem9_def)
+apply(intro allI impI)
+apply(simp (no_asm) add: fts_invariant_def)
+apply(intro allI impI, elim conjE)
+apply(rename_tac f ts f' ts')
+apply(intro conjI)
+ apply(force simp: fts_invariant_def)
+ 
+ (* focus_to_check_keys_2 *)
+ apply(simp add: focus_to_check_keys_2_def)
+ apply(subgoal_tac "?  k xs l t u zs. f = Focus(k,xs,l,t,u,zs)") prefer 2 apply(force intro:FIXME)
+ apply(elim exE, simp)
+ apply(subgoal_tac "? k' xs' l' t' u' zs'. f' = Focus(k',xs',l',t',u',zs')") prefer 2 apply(force intro:FIXME)
+ apply(elim exE, simp)
+ apply(simp add: step_fts_def)
+ apply(case_tac t) prefer 2 apply(force)
+ apply(simp)
+ apply(case_tac x1) apply(simp) apply(rename_tac ks rs)
+ apply(subgoal_tac "
+   ? i cn ts2 t2 l2 u2.
+   (search_key_to_index ks k = i) &
+    (Cnode(xs,l,ks,rs,i,u,zs) = cn) &
+    ((cn # ts2) = ts) &
+    (rs!i = t2) &
+    (cnode_to_bound cn = (l2,u2)) 
+
+") prefer 2 apply(force intro:FIXME)
+ apply(elim exE conjE)
+ apply(simp add: Let_def)
+ apply(elim conjE)
+ apply(simp add: check_keys_2_def)
+ (* and these are all fairly easy - see lem 7 below *)
+ apply(force intro:FIXME)
+ 
+ 
+ (* focus_to_leaves - this requires much the same sort of reasoning, so FIXME we should be able to combine with above? *)
+ apply(subgoal_tac "?  k xs l t u zs. f = Focus(k,xs,l,t,u,zs)") prefer 2 apply(force intro:FIXME)
+ apply(elim exE, simp)
+ apply(subgoal_tac "? k' xs' l' t' u' zs'. f' = Focus(k',xs',l',t',u',zs')") prefer 2 apply(force intro:FIXME)
+ apply(elim exE, simp)
+ apply(simp add: focus_to_leaves_def)
+ apply(drule_tac t=ls in sym) apply(simp)
+ apply(clarsimp)
+ apply(simp add: step_fts_def)
+ apply(case_tac t) prefer 2 apply(force)
+ apply(simp)
+ apply(case_tac x1) apply(simp) apply(rename_tac ks rs)
+ apply(subgoal_tac "
+   ? i cn ts2 t2 l2 u2.
+   (search_key_to_index ks k = i) &
+    (Cnode(xs,l,ks,rs,i,u,zs) = cn) &
+    ((cn # ts2) = ts) &
+    (rs!i = t2) &
+    (cnode_to_bound cn = (l2,u2)) 
+
+") prefer 2 apply(force intro:FIXME)
+ apply(elim exE conjE)
+ apply(simp add: Let_def)
+ apply(elim conjE)
+ apply(drule_tac t=i in sym) apply(simp)
+ (* and this is just a lemma about tree_to_leaves on a node *)
+ apply(simp add: tree_to_leaves_node_eq)
+ apply(drule_tac t=xs' in sym) apply(simp)
+ apply(drule_tac t=zs' in sym) apply(simp)
+ apply(drule_tac s=i in sym) apply(simp)
+ apply(drule_tac t=t' in sym) apply(simp)
+ apply(subgoal_tac "rs |> map tree_to_leaves = (
+   let rsi = % i. rs!i in
+   let xs = (from_to 0 (i-1))|> List.map rsi in
+   let ys = [i] |> List.map rsi in
+   let zs = (from_to (i+1) (ks_to_max_child_index ks)) |> List.map rsi in
+   (xs@ys@zs) |> map tree_to_leaves)")
+  prefer 2 apply(force intro: FIXME)
+ apply(simp add: Let_def)
+ apply(simp add: rev_apply_def)
+ apply(simp add: indexes_to_leaves_def)
+ apply(simp add: rev_apply_def)
+ apply(subgoal_tac "tree_to_leaves o (op ! rs) = (% j. let r = tree_to_leaves (rs!j) in r)") prefer 2 apply(force intro: FIXME)
+ apply(force)
+ done
+
 lemma "lem7"
 apply(simp add: lem7_def) 
 apply(intro allI)
